Fix a bug in extraction of  singleton elimination:
We need to add boxes for the pattern-matching branches arguments.

extraction/test-suite/Test.v
@@ -40,3 +40,141 @@ Eval cbv in extract_term (types_env, len).
 Program Definition exn : { x : nat | x > 0 } := 1.
 Quote Recursively Definition exn_ast := exn.
 Eval cbv in extract exn_ast.
+
+Require Import Coq.Arith.Wf_nat.
+Require Import Recdef.
+
+Function provedCopy (n:nat) {wf lt n} :=
+  match n with 0 => 0 | S k => S (provedCopy k) end.
+Proof.
+  - intros. constructor.
+  - apply lt_wf.
+Defined.
+
+Quote Recursively Definition copy := provedCopy.
+
+(* Quote Recursively Definition copy_types := (nat, bool, list, List.length, sig, fun A B => prod A B, gt, le, Acc, ex, eq). *)
+(* Definition copy_types_env := fst copy_types. *)
+Require Import ETyping.
+
+Definition extract_copy := Eval native_compute in extract copy.
+
+Require Import EAst.
+Section PP.
+Require Import Coq.Arith.Div2 Coq.Numbers.Natural.Peano.NPeano Coq.Program.Wf.
+Local Open Scope string_scope.
+
+Definition digit_to_string (n:nat): string :=
+  match n with
+    | 0 => "0" | 1 => "1" | 2 => "2" | 3 => "3" | 4 => "4"
+    | 5 => "5" | 6 => "6" | 7 => "7" | 8 => "8" | _ => "9"
+  end%nat.
+
+Program Fixpoint nat_to_string (n:nat) {measure n}: string :=
+  (match n <? 10 as x return n <? 10 = x -> string with
+     | true => fun _ => digit_to_string n
+     | false => fun pf =>
+                  let m := NPeano.Nat.div n 10 in
+                  (nat_to_string m) ++ (digit_to_string (n - 10 * m))
+   end eq_refl)%nat.
+Next Obligation.
+  apply (NPeano.Nat.div_lt n 10%nat).
+  destruct n. unfold NPeano.Nat.ltb in *. simpl in *.
+  discriminate. auto with arith.
+  auto with arith.
+Defined.
+
+End PP.
+(** Printing terms in exceptions for debugging purposes **)
+Definition print_name nm : string :=
+  match nm with
+  | nAnon => " _ "
+  | nNamed str => str
+  end.
+Definition print_inductive (i:inductive) : string :=
+  match i with
+  | mkInd str n => ("(inductive:" ++ str ++ ":" ++ nat_to_string n ++ ")")
+  end.
+
+Require Import Ascii.
+Definition newline_char := "010"%char.
+Definition newline : string := String newline_char EmptyString.
+
+Definition nth_error {A} : forall (l : list A) (n : nat), option A :=
+  fix aux l n :=
+  match l with
+  | nil => None
+  | cons x xs => match n with
+                 | 0 => Some x
+                 | S n => aux xs n
+                 end
+  end.
+
+Fixpoint print_extracted_term (t:term) (names : list name) (inapp : bool) : string :=
+  match t with
+  | tBox => "⧆"
+  | tVar id => "Var(" ++ id ++ ")"
+  | tMeta n => "Meta(" ++ nat_to_string n ++ ")"
+  | tEvar n e => "Evar"
+  | tRel n =>
+    match List.nth_error names n with
+    | None | Some nAnon => " (" ++ (nat_to_string n) ++ ") "
+    | Some (nNamed str) => str
+    end
+  | tLambda na t => "(LAM " ++ (print_name na) ++ "," ++ print_extracted_term t (na :: names) true ++ ")"
+  | tLetIn na b t => "(LET " ++ (print_name na) ++ ":=" ++ print_extracted_term b names true ++ " in " ++ newline ++
+                             print_extracted_term t (na :: names) true ++ ")"
+  | tApp fn arg =>
+    if inapp then print_extracted_term fn names true ++ " " ++ print_extracted_term arg names false
+    else
+      " (" ++ (print_extracted_term fn names true) ++ " " ++ print_extracted_term arg names false ++ ") "
+  | tConst s => "[" ++ s ++ "]"
+  | tConstruct i n =>
+    "(CSTR:" ++ print_inductive i ++ ":" ++ (nat_to_string n) ++ ") "
+  | tCase n mch brs =>
+    let brs :=
+        let fix aux l :=
+            match l with
+            | nil => ""
+            | cons x xs => print_extracted_term (snd x) names true ++ newline ++ aux xs
+            end
+        in aux brs
+    in
+    " (match " ++ (print_extracted_term mch names true) ++ " in " ++ print_inductive (fst n) ++ "," ++ (nat_to_string (snd n)) ++ " with " ++ newline ++
+               brs ++ "end)" ++ newline
+  | tProj (ind, nargs, n) c => print_extracted_term c names false ++ ".(" ++ nat_to_string n ++ ")"
+  | tFix bds n =>
+    let names := (List.map (fun d => d.(dname)) bds ++ names)%list in
+    " (FIX " ++ (nat_to_string n) ++ " " ++
+                           let fix aux l n :=
+    match l with
+    | nil => ""
+    | cons x xs => match n with
+                   | 0 => print_name x.(dname) ++ " { " ++ "struct " ++ nat_to_string x.(rarg) ++ "} " ++
+                                                                      print_extracted_term x.(dbody) names true
+                   | S n => aux xs n
+                   end
+    end in aux bds n ++ ") "
+  | tCoFix _ n => " (COFIX " ++ (nat_to_string n) ++ ") "
+  end.
+
+Set Printing Depth 10000.
+
+Definition print_def c :=
+  match extract_copy with
+  | Some (env, term) =>
+    match lookup_env env c with
+    | Some (ConstantDecl _ cb) =>
+      match cb.(cst_body) with
+      | Some b => print_extracted_term b nil true
+      | None => "an axiom"
+      end
+    | Some (InductiveDecl _ _) =>
+      "an inductive"
+    | None => "not found in the environment"
+    end
+  | None => "nothing"
+  end.
+
+Eval cbv in print_def "Top.provedCopy_terminate".
+Eval cbv in print_def "Coq.Init.Logic.and_rect".
